save dep interpreter (inefficient)

shift-reset/core/syntax.v
@@ -2,8 +2,8 @@ From Stdlib Require Import Bool ZArith.
 From shift_reset.core Require Import loc var.
 
 Inductive prim1 : Type :=
-| P1Neg : prim1
-| P1Not : prim1.
+| P1Not : prim1
+| P1Neg : prim1.
 
 Inductive prim2 : Type :=
 | P2Add : prim2
@@ -11,40 +11,33 @@ Inductive prim2 : Type :=
 | P2Mul : prim2
 | P2Div : prim2
 | P2Rem : prim2
+| P2Lt : prim2
+| P2Le : prim2
 | P2And : prim2
 | P2Or : prim2
 | P2Xor : prim2
 | P2Eq : prim2
-| P2Lt : prim2
-| P2Le : prim2.
+| P2Neq : prim2.
 
 Inductive binder : Type :=
 | BAnon : binder
 | BVar : var -> binder.
 
-Inductive val : Type :=
-| VUnit : val
-| VBool : bool -> val
-| VInt : Z -> val
-| VFun : clo1 -> val
-| VFix : clo2 -> val
-| VPair : val -> val -> val
-| VInl : val -> val
-| VInr : val -> val
-| VLoc : loc -> val
-| VKont : kont -> val
-with atom : Type :=
-| AVal : val -> atom
-| AVar : var -> atom
-with term : Type :=
+Inductive atom : Type :=
+| AUnit : atom
+| AInt : Z -> atom
+| ABool : bool -> atom
+| AVar : var -> atom.
+
+Inductive term : Type :=
 | TAtom : atom -> term
+| TFun : term1 -> term
+| TFix : term2 -> term
+| TApp : atom -> atom -> term
 | TLet : term -> term1 -> term
 | TIf : atom -> term -> term -> term
 | TPrim1 : prim1 -> atom -> term
 | TPrim2 : prim2 -> atom -> atom -> term
-| TFun : term1 -> term
-| TFix : term2 -> term
-| TApp : atom -> atom -> term
 | TPair : atom -> atom -> term
 | TFst : atom -> term
 | TSnd : atom -> term
@@ -57,15 +50,26 @@ with term : Type :=
 | TFree : atom -> term
 | TShift : term1 -> term
 | TReset : term -> term
-| TCont : term -> clo1 -> term
 with term1 : Type :=
 | T1 : binder -> term -> term1
 with term2 : Type :=
-| T2 : binder -> term1 -> term2
+| T2 : binder -> term1 -> term2.
+
+Inductive val : Type :=
+| VUnit : val
+| VInt : Z -> val
+| VBool : bool -> val
+| VFun : clo1 -> val
+| VFix : clo2 -> val
+| VPair : val -> val -> val
+| VInl : val -> val
+| VInr : val -> val
+| VLoc : loc -> val
+| VKont : kont -> val
 with clo1 : Type :=
-| C1 : term1 -> env -> clo1
+| C1 : env -> term1 -> clo1
 with clo2 : Type :=
-| C2 : term2 -> env -> clo2
+| C2 : env -> term2 -> clo2
 with kont : Type :=
 | KNil : kont
 | KCons : clo1 -> kont -> kont
@@ -82,36 +86,38 @@ Proof. decide equality. Defined.
 Definition binder_eq_dec : forall (b1 b2 : binder), {b1 = b2} + {b1 <> b2}.
 Proof. decide equality; auto using var_eq_dec. Defined.
 
-Fixpoint val_eq_dec : forall (v1 v2 : val), {v1 = v2} + {v1 <> v2}
-with atom_eq_dec : forall (a1 a2 : atom), {a1 = a2} + {a1 <> a2}
-with term_eq_dec : forall (t1 t2 : term), {t1 = t2} + {t1 <> t2}
+Definition atom_eq_dec : forall (a1 a2 : atom), {a1 = a2} + {a1 <> a2}.
+Proof. decide equality; auto using Z.eq_dec, bool_dec, var_eq_dec. Defined.
+
+Fixpoint term_eq_dec : forall (t1 t2 : term), {t1 = t2} + {t1 <> t2}
 with term1_eq_dec : forall (t1 t2 : term1), {t1 = t2} + {t1 <> t2}
-with term2_eq_dec : forall (t1 t2 : term2), {t1 = t2} + {t1 <> t2}
+with term2_eq_dec : forall (t1 t2 : term2), {t1 = t2} + {t1 <> t2}.
+Proof.
+  { decide equality; auto using atom_eq_dec, prim1_eq_dec, prim2_eq_dec. }
+  { decide equality; auto using binder_eq_dec. }
+  { decide equality; auto using binder_eq_dec. }
+Defined.
+
+Fixpoint val_eq_dec : forall (v1 v2 : val), {v1 = v2} + {v1 <> v2}
 with clo1_eq_dec : forall (c1 c2 : clo1), {c1 = c2} + {c1 <> c2}
 with clo2_eq_dec : forall (c1 c2 : clo2), {c1 = c2} + {c1 <> c2}
 with kont_eq_dec : forall (k1 k2 : kont), {k1 = k2} + {k1 <> k2}
 with env_eq_dec : forall (env1 env2 : env), {env1 = env2} + {env1 <> env2}.
 Proof.
-  { decide equality; auto using bool_dec, Z.eq_dec, loc_eq_dec. }
-  { decide equality; auto using var_eq_dec. }
-  { decide equality; auto using prim1_eq_dec, prim2_eq_dec. }
-  { decide equality; auto using binder_eq_dec. }
-  { decide equality; auto using binder_eq_dec. }
-  { decide equality. }
-  { decide equality. }
+  { decide equality; auto using Z.eq_dec, bool_dec, loc_eq_dec. }
+  { decide equality; auto using term1_eq_dec. }
+  { decide equality; auto using term2_eq_dec. }
   { decide equality. }
   { decide equality; auto using var_eq_dec. }
 Defined.
 
-Definition val_eqb (v1 v2 : val) : bool := if val_eq_dec v1 v2 then true else false.
-Definition term_eqb (t1 t2 : term) : bool := if term_eq_dec t1 t2 then true else false.
+Definition val_eqb (v1 v2 : val) : bool := proj1_sig (bool_of_sumbool (val_eq_dec v1 v2)).
+Definition val_neqb (v1 v2 : val) : bool := negb (val_eqb v1 v2).
 
 Module Coerce.
   Coercion BVar : var >-> binder.
-  Coercion VBool : bool >-> val.
-  Coercion VInt : Z >-> val.
-  Coercion VLoc : loc >-> val.
-  Coercion AVal : val >-> atom.
+  Coercion AInt : Z >-> atom.
+  Coercion ABool : bool >-> atom.
   Coercion AVar : var >-> atom.
   Coercion TAtom : atom >-> term.
 End Coerce.
