shift-reset/interpreter/interpreter.v
@@ -3,16 +3,18 @@ From shift_reset.core Require Import syntax var env.
 From shift_reset.interpreter Require Import istate ierror imonad.
 
 Local Open Scope string_scope.
-Local Open Scope Z_scope.
 
 Definition interpret_atom (a : atom) : imonad val :=
   match a with
-  | AVal v => imonad_pure v
-  | AVar x => imonad_bind imonad_ask_env
-                (fun env => match env_lookup x env with
-                            | None => imonad_throw (NameError "")
-                            | Some v => imonad_pure v
-                            end)
+  | AUnit => imonad_pure VUnit
+  | AInt i => imonad_pure (VInt i)
+  | ABool b => imonad_pure (VBool b)
+  | AVar x =>
+      imonad_bind imonad_ask_env
+        (fun env => match env_lookup x env with
+                    | None => imonad_throw (NameError "")
+                    | Some v => imonad_pure v
+                    end)
   end.
 
 Definition interpret_term1_aux (go : term -> imonad val) (t : term1) (v : val) : imonad val :=
@@ -30,28 +32,19 @@ Definition interpret_term2_aux (go : term -> imonad val) (t : term2) (v1 v2 : va
   end.
 
 Definition interpret_clo1_aux (go : term -> imonad val) (c : clo1) (v : val) : imonad val :=
-  let (t, env) := c in imonad_local_env (fun _ => env) (interpret_term1_aux go t v).
+  let (env, t) := c in imonad_local_env (fun _ => env) (interpret_term1_aux go t v).
 
 Definition interpret_clo2_aux (go : term -> imonad val) (c : clo2) (v1 v2 : val) : imonad val :=
-  let (t, env) := c in imonad_local_env (fun _ => env) (interpret_term2_aux go t v1 v2).
+  let (env, t) := c in imonad_local_env (fun _ => env) (interpret_term2_aux go t v1 v2).
 
-(*
-Definition interpret_kont_aux (go : kont -> term -> imonad val) (k : kont) (v : val) : imonad val :=
-  match k with
-  | KNil => imonad_pure v
-  | KCons c k' => interpret_clo1_aux (go k') c v
-  end.
-*)
-
-Definition interpret_let : imonad val -> (val -> imonad val) -> imonad val :=
-  imonad_bind.
-
-Definition interpret_if (a : atom) (t1 t2 : imonad val) :=
+Definition interpret_if (a : atom) (m1 m2 : imonad val) :=
   imonad_bind (interpret_atom a)
     (fun v => match v with
-              | VBool b => if b then t1 else t2
+              | VBool b => if b then m1 else m2
               | _ => imonad_throw (TypeError "")
               end).
+
+Local Open Scope Z_scope.
 
 Definition interpret_prim1 (p : prim1) (a : atom) : imonad val :=
   imonad_bind (interpret_atom a)
@@ -61,85 +54,84 @@ Definition interpret_prim1 (p : prim1) (a : atom) : imonad val :=
               | _, _ => imonad_throw (TypeError "")
               end).
 
-Definition interpret_prim2_aux (p : prim2) (a1 a2 : imonad val) : imonad val :=
-  imonad_bind a1
+Definition interpret_prim2 (p : prim2) (a1 a2 : atom) : imonad val :=
+  let m1 := interpret_atom a1 in
+  let m2 := interpret_atom a2 in
+  imonad_bind m1
     (fun v1 =>
        match p, v1 with
-       | P2Add, VInt i1 => imonad_bind a2
-                             (fun v2 => match v2 with
-                                        | VInt i2 => imonad_pure (VInt (i1 + i2))
-                                        | _ => imonad_throw (TypeError "")
-                                        end)
-       | P2Sub, VInt i1 => imonad_bind a2
-                             (fun v2 => match v2 with
-                                        | VInt i2 => imonad_pure (VInt (i1 - i2))
-                                        | _ => imonad_throw (TypeError "")
-                                        end)
-       | P2Mul, VInt i1 => imonad_bind a2
-                             (fun v2 => match v2 with
-                                        | VInt i2 => imonad_pure (VInt (i1 * i2))
-                                        | _ => imonad_throw (TypeError "")
-                                        end)
-       | P2Div, VInt i1 => imonad_bind a2
-                             (fun v2 => match v2 with
-                                        | VInt i2 => imonad_pure (VInt (i1 / i2))
-                                        | _ => imonad_throw (TypeError "")
-                                        end)
-       | P2Rem, VInt i1 => imonad_bind a2
-                             (fun v2 => match v2 with
-                                        | VInt i2 => imonad_pure (VInt (Z.rem i1 i2))
-                                        | _ => imonad_throw (TypeError "")
-                                        end)
-       | P2And, VBool b1 => imonad_bind a2
-                              (fun v2 => match v2 with
-                                         | VBool b2 => imonad_pure (VBool (b1 && b2))
-                                         | _ => imonad_throw (TypeError "")
-                                         end)
-       | P2Or, VBool b1 => imonad_bind a2
-                             (fun v2 => match v2 with
-                                        | VBool b2 => imonad_pure (VBool (b1 || b2))
-                                        | _ => imonad_throw (TypeError "")
-                                        end)
-       | P2Xor, VBool b1 => imonad_bind a2
-                              (fun v2 => match v2 with
-                                         | VBool b2 => imonad_pure (VBool (xorb b1 b2))
-                                         | _ => imonad_throw (TypeError "")
-                                         end)
-       | P2Eq, _ => imonad_bind a2 (fun v2 => imonad_pure (VBool (val_eqb v1 v2)))
-       | P2Lt, VInt i1 => imonad_bind a2
-                            (fun v2 => match v2 with
-                                       | VInt i2 => imonad_pure (VBool (i1 <? i2))
-                                       | _ => imonad_throw (TypeError "")
-                                       end)
-       | P2Le, VInt i1 => imonad_bind a2
-                            (fun v2 => match v2 with
-                                       | VInt i2 => imonad_pure (VBool (i1 <=? i2))
-                                       | _ => imonad_throw (TypeError "")
-                                       end)
+       | P2Add, VInt i1 =>
+           imonad_bind m2
+             (fun v2 => match v2 with
+                        | VInt i2 => imonad_pure (VInt (i1 + i2))
+                        | _ => imonad_throw (TypeError "")
+                        end)
+       | P2Sub, VInt i1 =>
+           imonad_bind m2
+             (fun v2 => match v2 with
+                        | VInt i2 => imonad_pure (VInt (i1 - i2))
+                        | _ => imonad_throw (TypeError "")
+                        end)
+       | P2Mul, VInt i1 =>
+           imonad_bind m2
+             (fun v2 => match v2 with
+                        | VInt i2 => imonad_pure (VInt (i1 * i2))
+                        | _ => imonad_throw (TypeError "")
+                        end)
+       | P2Div, VInt i1 =>
+           imonad_bind m2
+             (fun v2 => match v2 with
+                        | VInt i2 => imonad_pure (VInt (i1 / i2))
+                        | _ => imonad_throw (TypeError "")
+                        end)
+       | P2Rem, VInt i1 =>
+           imonad_bind m2
+             (fun v2 => match v2 with
+                        | VInt i2 => imonad_pure (VInt (Z.rem i1 i2))
+                        | _ => imonad_throw (TypeError "")
+                        end)
+       | P2Lt, VInt i1 =>
+           imonad_bind m2
+             (fun v2 => match v2 with
+                        | VInt i2 => imonad_pure (VBool (i1 <? i2))
+                        | _ => imonad_throw (TypeError "")
+                        end)
+       | P2Le, VInt i1 =>
+           imonad_bind m2
+             (fun v2 => match v2 with
+                        | VInt i2 => imonad_pure (VBool (i1 <=? i2))
+                        | _ => imonad_throw (TypeError "")
+                        end)
+       | P2And, VBool b1 =>
+           imonad_bind m2
+             (fun v2 => match v2 with
+                        | VBool b2 => imonad_pure (VBool (b1 && b2))
+                        | _ => imonad_throw (TypeError "")
+                        end)
+       | P2Or, VBool b1 =>
+           imonad_bind m2
+             (fun v2 => match v2 with
+                        | VBool b2 => imonad_pure (VBool (b1 || b2))
+                        | _ => imonad_throw (TypeError "")
+                        end)
+       | P2Xor, VBool b1 =>
+           imonad_bind m2
+             (fun v2 => match v2 with
+                        | VBool b2 => imonad_pure (VBool (xorb b1 b2))
+                        | _ => imonad_throw (TypeError "")
+                        end)
+       | P2Eq, _ => imonad_bind m2 (fun v2 => imonad_pure (VBool (val_eqb v1 v2)))
+       | P2Neq, _ => imonad_bind m2 (fun v2 => imonad_pure (VBool (val_neqb v1 v2)))
        | _, _ => imonad_throw (TypeError "")
        end).
 
-Definition interpret_prim2 (p : prim2) (a1 a2 : atom) : imonad val :=
-  interpret_prim2_aux p (interpret_atom a1) (interpret_atom a2).
+Local Close Scope Z_scope.
 
 Definition interpret_fun (t : term1) : imonad val :=
-  imonad_map (fun env => VFun (C1 t env)) imonad_ask_env.
+  imonad_map (fun env => VFun (C1 env t)) imonad_ask_env.
 
 Definition interpret_fix (t : term2) : imonad val :=
-  imonad_map (fun env => VFix (C2 t env)) imonad_ask_env.
-
-Definition interpret_app_aux (go : term -> imonad val) (a1 a2 : imonad val) : imonad val :=
-  imonad_bind a1
-    (fun v1 =>
-       match v1 with
-       | VFun c => imonad_bind a2 (interpret_clo1_aux go c)
-       | VFix c => imonad_bind a2 (interpret_clo2_aux go c v1)
-       | VKont k => imonad_throw (ControlError "VKont to be implemented")
-       | _ => imonad_throw (TypeError "")
-       end).
-
-Definition interpret_app (go : term -> imonad val) (a1 a2 : atom) : imonad val :=
-  interpret_app_aux go (interpret_atom a1) (interpret_atom a2).
+  imonad_map (fun env => VFix (C2 env t)) imonad_ask_env.
 
 Definition interpret_pair (a1 a2 : atom) : imonad val :=
   imonad_lift2 VPair (interpret_atom a1) (interpret_atom a2).
@@ -196,12 +188,14 @@ Definition interpret_get (a : atom) : imonad val :=
        | _ => imonad_throw (TypeError "")
        end).
 
-Definition interpret_set_aux (a1 a2 : imonad val) : imonad val :=
-  imonad_bind a1
+Definition interpret_set (a1 a2 : atom) : imonad val :=
+  let m1 := interpret_atom a1 in
+  let m2 := interpret_atom a2 in
+  imonad_bind m1
     (fun v1 =>
        match v1 with
        | VLoc l =>
-           imonad_bind a2
+           imonad_bind m2
              (fun v2 =>
                 imonad_bind imonad_get_state
                   (fun s =>
@@ -211,9 +205,6 @@ Definition interpret_set_aux (a1 a2 : imonad val) : imonad val :=
                      end))
        | _ => imonad_throw (TypeError "")
        end).
-
-Definition interpret_set (a1 a2 : atom) : imonad val :=
-  interpret_set_aux (interpret_atom a1) (interpret_atom a2).
 
 Definition interpret_free (a : atom) : imonad val :=
   imonad_bind (interpret_atom a)
@@ -240,8 +231,7 @@ Fixpoint term_size (t : term) : nat :=
   end
 with term1_size (t : term1) : nat := let (_, t') := t in term_size t'.
 
-Definition clo1_size (c : clo1) : nat :=
-  let (t, _) := c in term1_size t.
+Definition clo1_size (c : clo1) : nat := let (_, t) := c in term1_size t.
 
 Fixpoint kont_size (k : kont) : nat :=
   match k with
@@ -251,125 +241,261 @@ Fixpoint kont_size (k : kont) : nat :=
 
 Local Open Scope nat_scope.
 
-Definition interpret_term1_kont_aux (go : forall (t : term) (k : kont), Acc lt (term_size t + kont_size k) -> imonad val) (t : term1) (v : val) (k : kont) :
-  Acc lt (term1_size t + kont_size k) -> imonad val :=
-  match t with
-  | T1 b t' => fun H_acc =>
-                 let m := go t' k H_acc in
-                 match b with
-                 | BAnon => m
-                 | BVar x => imonad_local_env (ECons x v) m
-                 end
-  end.
+Section interpret_kont.
+  Context (go : forall (t : term) (k : kont), Acc lt (term_size t + kont_size k) -> imonad val).
 
-Definition interpret_clo1_kont_aux (go : forall (t : term) (k : kont), Acc lt (term_size t + kont_size k) -> imonad val) (c : clo1) (v : val) (k : kont) :
-  Acc lt (clo1_size c + kont_size k) -> imonad val :=
-  match c with C1 t env => fun H_acc => imonad_local_env (fun _ => env) (interpret_term1_kont_aux go t v k H_acc) end.
+  Definition interpret_term1_kont_aux (t : term1) (k : kont) (H_acc : Acc lt (term1_size t + kont_size k)) (v : val) : imonad val :=
+    match t return Acc lt (term1_size t + kont_size k) -> imonad val with
+    | T1 b t' => fun H_acc =>
+                   let m := go t' k H_acc in
+                   match b with
+                   | BAnon => m
+                   | BVar x => imonad_local_env (ECons x v) m
+                   end
+    end H_acc.
 
-Definition interpret_kont_aux (go : forall (t : term) (k : kont), Acc lt (term_size t + kont_size k) -> imonad val) (k : kont) (m : imonad val) :
-  Acc lt (kont_size k) -> imonad val :=
-  match k with
-  | KNil => fun _ => m
-  | KCons c k' => fun H_acc => imonad_bind m (fun v => interpret_clo1_kont_aux go c v k' H_acc)
-  end.
+  Definition interpret_clo1_kont_aux (c : clo1) (k : kont) (H_acc : Acc lt (clo1_size c + kont_size k)) (v : val) : imonad val :=
+    match c return Acc lt (clo1_size c + kont_size k) -> imonad val with
+    | C1 env t => fun H_acc => imonad_local_env (fun _ => env) (interpret_term1_kont_aux t k H_acc v)
+    end H_acc.
 
-Definition interpret_kont_aux' (go : term -> kont -> imonad val) (k : kont) (m : imonad val) : imonad val :=
+  Definition interpret_kont_aux (k : kont) (H_acc : Acc lt (kont_size k)) (m : imonad val) : imonad val :=
+    match k return Acc lt (kont_size k) -> imonad val with
+    | KNil => fun _ => m
+    | KCons c k' => fun H_acc => imonad_bind m (interpret_clo1_kont_aux c k' H_acc)
+    end H_acc.
+End interpret_kont.
+
+Definition interpret_kont (go : term -> kont -> imonad val) (k : kont) (m : imonad val) : imonad val :=
   match k with
   | KNil => m
   | KCons c k' => imonad_bind m (interpret_clo1_aux (fun t => go t k') c)
   end.
 
-Definition interpret_term_kont_aux (go : term -> kont -> imonad val) (t : term) (k : kont) : imonad val.
-  refine ((fix go' t k (H_acc : Acc lt (term_size t + kont_size k)) {struct H_acc} : imonad val :=
-             match t return Acc lt (term_size t + kont_size k) -> imonad val with
-             | TAtom a => fun H_acc => interpret_kont_aux go' k (interpret_atom a) _
-             | TLet t1 t2 => fun H_acc => imonad_bind imonad_ask_env (fun env => go' t1 (KCons (C1 t2 env) k) _)
-             | TIf a t1 t2 => fun H_acc => interpret_if a (go' t1 k _) (go' t2 k _)
-             | TPrim1 p a => fun H_acc => interpret_kont_aux go' k (interpret_prim1 p a) _
-             | TPrim2 p a1 a2 => fun H_acc => interpret_kont_aux go' k (interpret_prim2 p a1 a2) _
-             | TFun t' => fun H_acc => interpret_kont_aux go' k (interpret_fun t') _
-             | TFix t' => fun H_acc => interpret_kont_aux go' k (interpret_fix t') _
-             | TApp a1 a2 => fun _ => interpret_app (fun t' => go t' k) a1 a2
-             | TPair a1 a2 => fun H_acc => interpret_kont_aux go' k (interpret_pair a1 a2) _
-             | TFst a => fun H_acc => interpret_kont_aux go' k (interpret_fst a) _
-             | TSnd a => fun H_acc => interpret_kont_aux go' k (interpret_snd a) _
-             | TInl a => fun H_acc => interpret_kont_aux go' k (interpret_inl a) _
-             | TInr a => fun H_acc => interpret_kont_aux go' k (interpret_inr a) _
-             | TCase a t1 t2 => fun H_acc => interpret_case a
-                                               (fun v => interpret_term1_kont_aux go' t1 v k _)
-                                               (fun v => interpret_term1_kont_aux go' t2 v k _)
-             | TShift t' => fun H_acc => interpret_term1_kont_aux go' t' (VKont k) KNil _
-             | TReset t' => fun H_acc => interpret_kont_aux go' k (go' t' KNil _) _
-             | _ => fun _ => imonad_throw OutOfFuel
-             end H_acc) t k (lt_wf _)).
-  - simpl in *. apply (Acc_inv H_acc). lia.
-  - simpl in *. apply (Acc_inv H_acc). lia.
-  - simpl in *. apply (Acc_inv H_acc). lia.
-  - simpl in *. apply (Acc_inv H_acc). lia.
-  - simpl in *. apply (Acc_inv H_acc). lia.
-  - simpl in *. apply (Acc_inv H_acc). lia.
-  - simpl in *. apply (Acc_inv H_acc). lia.
-  - simpl in *. apply (Acc_inv H_acc). lia.
-  - simpl in *. apply (Acc_inv H_acc). lia.
-  - simpl in *. apply (Acc_inv H_acc). lia.
-  - simpl in *. apply (Acc_inv H_acc). lia.
-  - simpl in *. apply (Acc_inv H_acc). lia.
-  - simpl in *. apply (Acc_inv H_acc). lia.
-  - simpl in *. apply (Acc_inv H_acc). lia.
-  - simpl in *. apply (Acc_inv H_acc). lia.
-  - simpl in *. apply (Acc_inv H_acc). lia.
-  - simpl in *. apply (Acc_inv H_acc). lia.
-  - simpl in *. apply (Acc_inv H_acc). lia.
+Lemma Acc_inv_succ (n : nat) (H_acc : Acc lt (S n)) : Acc lt n.
+Proof.
+  apply (Acc_inv H_acc).
+  exact (Nat.lt_succ_diag_r n).
 Defined.
 
-Local Close Scope nat_scope.
+Lemma Acc_inv_succ_add (m n : nat) (H_acc : Acc lt (S (m + n))) : Acc lt n.
+Proof.
+  apply (Acc_inv H_acc).
+  rewrite -> Nat.lt_succ_r.
+  exact (Nat.le_add_l n m).
+Defined.
 
-Definition interpret_term_kont_bot (_ : term) (_ : kont) : imonad val :=
-  imonad_throw OutOfFuel.
+Lemma Acc_inv_succ_add_max_l (n m p : nat) (H_acc : Acc lt (S (Nat.max n m + p))) : Acc lt (n + p).
+Proof.
+  apply (Acc_inv H_acc).
+  rewrite -> Nat.lt_succ_r.
+  rewrite <- Nat.add_le_mono_r.
+  exact (Nat.le_max_l _ _).
+Defined.
+
+Lemma Acc_inv_succ_add_max_r (n m p : nat) (H_acc : Acc lt (S (Nat.max n m + p))) : Acc lt (m + p).
+Proof.
+  apply (Acc_inv H_acc).
+  rewrite -> Nat.lt_succ_r.
+  rewrite <- Nat.add_le_mono_r.
+  exact (Nat.le_max_r _ _).
+Defined.
+
+Lemma Acc_inv_succ_add0 (m n : nat) (H_acc : Acc lt (S (m + n))) : Acc lt (m + 0).
+Proof.
+  apply (Acc_inv H_acc).
+  rewrite -> Nat.add_0_r.
+  rewrite -> Nat.lt_succ_r.
+  exact (Nat.le_add_r m n).
+Defined.
+
+(*
+Definition interpret_term_kont_aux (go : term -> kont -> imonad val) (t : term) (k : kont) : imonad val.
+  refine
+    ((fix go' t k (H_acc : Acc lt (term_size t + kont_size k)) {struct H_acc} : imonad val :=
+        match t return Acc lt (term_size t + kont_size k) -> imonad val with
+        | TAtom a => fun H_acc => interpret_kont_aux go' k _ (interpret_atom a)
+        | TLet t1 t2 => fun H_acc => imonad_bind imonad_ask_env (fun env => go' t1 (KCons (C1 env t2) k) _)
+        | TIf a t1 t2 => fun H_acc => interpret_if a (go' t1 k _) (go' t2 k _)
+        | TPrim1 p a => fun H_acc => interpret_kont_aux go' k _ (interpret_prim1 p a)
+        | TPrim2 p a1 a2 => fun H_acc => interpret_kont_aux go' k _ (interpret_prim2 p a1 a2)
+        | TFun t' => fun H_acc => interpret_kont_aux go' k _ (interpret_fun t')
+        | TFix t' => fun H_acc => interpret_kont_aux go' k _ (interpret_fix t')
+        | TApp a1 a2 => fun H_acc =>
+                          let m1 := interpret_atom a1 in
+                          let m2 := interpret_atom a2 in
+                          imonad_bind m1
+                            (fun v1 =>
+                               match v1 with
+                               | VFun c => imonad_bind m2 (interpret_clo1_aux (fun t' => go t' k) c)
+                               | VFix c => imonad_bind m2 (interpret_clo2_aux (fun t' => go t' k) c v1)
+                               | VKont k' => interpret_kont_aux go' k _ (interpret_kont go k'  m2)
+                               | _ => imonad_throw (TypeError "")
+                               end)
+        | TPair a1 a2 => fun H_acc => interpret_kont_aux go' k _ (interpret_pair a1 a2)
+        | TFst a => fun H_acc => interpret_kont_aux go' k _ (interpret_fst a)
+        | TSnd a => fun H_acc => interpret_kont_aux go' k _ (interpret_snd a)
+        | TInl a => fun H_acc => interpret_kont_aux go' k _ (interpret_inl a)
+        | TInr a => fun H_acc => interpret_kont_aux go' k _ (interpret_inr a)
+        | TCase a t1 t2 => fun H_acc => interpret_case a (interpret_term1_kont_aux go' t1 k _) (interpret_term1_kont_aux go' t2 k _)
+        | TRef a => fun H_acc => interpret_kont_aux go' k _ (interpret_ref a)
+        | TGet a => fun H_acc => interpret_kont_aux go' k _ (interpret_get a)
+        | TSet a1 a2 => fun H_acc => interpret_kont_aux go' k _ (interpret_set a1 a2)
+        | TFree a => fun H_acc => interpret_kont_aux go' k _ (interpret_free a)
+        | TShift t' => fun H_acc => interpret_term1_kont_aux go' t' KNil _ (VKont k)
+        | TReset t' => fun H_acc => interpret_kont_aux go' k _ (go' t' KNil _)
+        end H_acc) t k (lt_wf _)).
+  - simpl in *. exact (Acc_inv_succ _ H_acc).
+  - simpl in *. exact (Acc_inv_succ _ H_acc).
+  - simpl in *. exact (Acc_inv_succ _ H_acc).
+  - simpl in *. exact (Acc_inv_succ _ H_acc).
+  - simpl in *. apply (Acc_inv H_acc). lia.
+  - simpl in *. exact (Acc_inv_succ_add_max_l _ _ _ H_acc).
+  - simpl in *. exact (Acc_inv_succ_add_max_r _ _ _ H_acc).
+  - simpl in *. exact (Acc_inv_succ _ H_acc).
+  - simpl in *. exact (Acc_inv_succ _ H_acc).
+  - simpl in *. exact (Acc_inv_succ _ H_acc).
+  - simpl in *. exact (Acc_inv_succ _ H_acc).
+  - simpl in *. exact (Acc_inv_succ _ H_acc).
+  - simpl in *. exact (Acc_inv_succ _ H_acc).
+  - simpl in *. exact (Acc_inv_succ _ H_acc).
+  - simpl in *. exact (Acc_inv_succ_add_max_l _ _ _ H_acc).
+  - simpl in *. exact (Acc_inv_succ_add_max_r _ _ _ H_acc).
+  - simpl in *. exact (Acc_inv_succ _ H_acc).
+  - simpl in *. exact (Acc_inv_succ _ H_acc).
+  - simpl in *. exact (Acc_inv_succ _ H_acc).
+  - simpl in *. exact (Acc_inv_succ _ H_acc).
+  - simpl in *. exact (Acc_inv_succ_add0 _ _ H_acc).
+  - simpl in *. exact (Acc_inv_succ_add _ _ H_acc).
+  - simpl in *. exact (Acc_inv_succ_add0 _ _ H_acc).
+Defined.
+*)
+
+Inductive tree :=
+| Nat : nat -> tree
+| Plus : tree -> tree -> tree.
+
+Fixpoint tree_size' t acc := match t with Nat _ => S acc | Plus t1 t2 => S (tree_size' t1 (tree_size' t2 acc)) end.
+Definition tree_size'' t := tree_size' t 0.
+Fixpoint tree_size t := match t with Nat _ => 1 | Plus t1 t2 => S (tree_size t1 + tree_size t2) end.
+Fixpoint list_size ts := match ts with nil => 0 | cons t ts' => tree_size'' t + list_size ts' end.
+
+Axiom equiv : forall t, tree_size'' t = tree_size t.
+Axiom equiv' : forall t acc, tree_size' t acc = tree_size t + acc.
+
+From Stdlib Require Import FunInd Recdef Program.
+
+Program Fixpoint sum_tree' (ts : list tree) (acc : nat) {measure (list_size ts)} :=
+  match ts with
+  | nil => acc
+  | cons t ts' =>
+      match t with
+      | Nat n => sum_tree' ts' (n + acc)
+      | Plus l r => sum_tree' (cons l (cons r ts')) acc
+      end
+  end.
+Next Obligation.
+  simpl.
+  rewrite ->! equiv.
+  rewrite ->! equiv'.
+  lia.
+Qed.
+
+Definition sum_tree t := sum_tree' (cons t nil) 0.
+
+Fixpoint sum_t' t acc :=
+  match t with
+  | Nat n => n + acc
+  | Plus l r => sum_t' r (sum_t' l acc)
+  end.
+
+Definition sum_t t := sum_t' t 0.
+
+Print sum_tree'_func.
+
+Fixpoint gen_large_tree (xs : list nat) :=
+  match xs with
+  | nil => Nat 1
+  | cons x xs' => Plus (gen_large_tree xs') (Nat 1)
+  end.
+
+Definition large := gen_large_tree (ListDef.seq 0 2000).
+
+Time Compute (sum_t large).
+Time Compute (sum_tree large).
+
+
+
+(*
+Section foo.
+Context (go : term -> kont -> imonad val).
+
+Program Fixpoint go' (t : term) (k : kont) {measure (term_size t + kont_size k)} : imonad val :=
+  match t with
+  | TAtom a => interpret_kont_aux go' k _ (interpret_atom a)
+  | TLet t1 t2 => fun H_acc => imonad_bind imonad_ask_env (fun env => go' t1 (KCons (C1 env t2) k) _)
+  (*
+  | TIf a t1 t2 => fun H_acc => interpret_if a (go' t1 k _) (go' t2 k _)
+  | TPrim1 p a => fun H_acc => interpret_kont_aux go' k _ (interpret_prim1 p a)
+  | TPrim2 p a1 a2 => fun H_acc => interpret_kont_aux go' k _ (interpret_prim2 p a1 a2)
+  | TFun t' => fun H_acc => interpret_kont_aux go' k _ (interpret_fun t')
+  | TFix t' => fun H_acc => interpret_kont_aux go' k _ (interpret_fix t')
+  | TApp a1 a2 => fun H_acc =>
+                    let m1 := interpret_atom a1 in
+                    let m2 := interpret_atom a2 in
+                    imonad_bind m1
+                      (fun v1 =>
+                         match v1 with
+                         | VFun c => imonad_bind m2 (interpret_clo1_aux (fun t' => go t' k) c)
+                         | VFix c => imonad_bind m2 (interpret_clo2_aux (fun t' => go t' k) c v1)
+                         | VKont k' => interpret_kont_aux go' k _ (interpret_kont go k'  m2)
+                         | _ => imonad_throw (TypeError "")
+                         end)*)
+  | TPair a1 a2 => fun H_acc => interpret_kont_aux go' k _ (interpret_pair a1 a2)
+  | TFst a => fun H_acc => interpret_kont_aux go' k _ (interpret_fst a)
+  | TSnd a => fun H_acc => interpret_kont_aux go' k _ (interpret_snd a)
+  | TInl a => fun H_acc => interpret_kont_aux go' k _ (interpret_inl a)
+  | TInr a => fun H_acc => interpret_kont_aux go' k _ (interpret_inr a)
+  | TCase a t1 t2 => fun H_acc => interpret_case a (interpret_term1_kont_aux go' t1 k _) (interpret_term1_kont_aux go' t2 k _)
+  | TRef a => fun H_acc => interpret_kont_aux go' k _ (interpret_ref a)
+  | TGet a => fun H_acc => interpret_kont_aux go' k _ (interpret_get a)
+  | TSet a1 a2 => fun H_acc => interpret_kont_aux go' k _ (interpret_set a1 a2)
+  | TFree a => fun H_acc => interpret_kont_aux go' k _ (interpret_free a)
+  | TShift t' => fun H_acc => interpret_term1_kont_aux go' t' KNil _ (VKont k)
+  | TReset t' => fun H_acc => interpret_kont_aux go' k _ (go' t' KNil _)
+  end.
+  - simpl in *. exact (Acc_inv_succ _ H_acc).
+  - simpl in *. exact (Acc_inv_succ _ H_acc).
+  - simpl in *. exact (Acc_inv_succ _ H_acc).
+  - simpl in *. exact (Acc_inv_succ _ H_acc).
+  - simpl in *. apply (Acc_inv H_acc). lia.
+  - simpl in *. exact (Acc_inv_succ_add_max_l _ _ _ H_acc).
+  - simpl in *. exact (Acc_inv_succ_add_max_r _ _ _ H_acc).
+  - simpl in *. exact (Acc_inv_succ _ H_acc).
+  - simpl in *. exact (Acc_inv_succ _ H_acc).
+  - simpl in *. exact (Acc_inv_succ _ H_acc).
+  - simpl in *. exact (Acc_inv_succ _ H_acc).
+  - simpl in *. exact (Acc_inv_succ _ H_acc).
+  - simpl in *. exact (Acc_inv_succ _ H_acc).
+  - simpl in *. exact (Acc_inv_succ _ H_acc).
+  - simpl in *. exact (Acc_inv_succ_add_max_l _ _ _ H_acc).
+  - simpl in *. exact (Acc_inv_succ_add_max_r _ _ _ H_acc).
+  - simpl in *. exact (Acc_inv_succ _ H_acc).
+  - simpl in *. exact (Acc_inv_succ _ H_acc).
+  - simpl in *. exact (Acc_inv_succ _ H_acc).
+  - simpl in *. exact (Acc_inv_succ _ H_acc).
+  - simpl in *. exact (Acc_inv_succ_add0 _ _ H_acc).
+  - simpl in *. exact (Acc_inv_succ_add _ _ H_acc).
+  - simpl in *. exact (Acc_inv_succ_add0 _ _ H_acc).
+Defined.
+*)
+Local Close Scope nat_scope.
 
 Fixpoint interpret_term_kont (fuel : nat) (t : term) (k : kont) : imonad val :=
   match fuel with
-  | O => interpret_term_kont_bot
-  | S fuel' => interpret_term_kont_aux (interpret_term_kont fuel')
-  end t k.
-
-(*
-Definition interpret_term_cont_aux (go : term -> imonad val) (go_cont : clo1 -> term -> imonad val) : clo1 -> term -> imonad val :=
-  fix go_cont' k t {struct t} :=
-    match t with
-    | TAtom a => imonad_bind (interpret_atom a) (interpret_clo1_aux go k)
-    | TLet t1 t2 => imonad_bind imonad_ask_env (fun env => go_cont' (C1 (compose t2 k) env) t1)
-    | TIf a t1 t2 => interpret_if a (go_cont' k t1) (go_cont' k t2)
-    | TPrim1 p a => imonad_bind (interpret_prim1 p a) (interpret_clo1_aux go k)
-    | TPrim2 p a1 a2 => imonad_bind (interpret_prim2 p a1 a2) (interpret_clo1_aux go k)
-    | TFun t' => imonad_bind (interpret_fun t') (interpret_clo1_aux go k)
-    | TFix t' => imonad_bind (interpret_fix t') (interpret_clo1_aux go k)
-    | TApp a1 a2 => interpret_app (go_cont k) a1 a2
-    | TPair a1 a2 => imonad_bind (interpret_pair a1 a2) (interpret_clo1_aux go k)
-    | TFst a => imonad_bind (interpret_fst a) (interpret_clo1_aux go k)
-    | TSnd a => imonad_bind (interpret_snd a) (interpret_clo1_aux go k)
-    | TInl a => imonad_bind (interpret_inl a) (interpret_clo1_aux go k)
-    | TInr a => imonad_bind (interpret_inr a) (interpret_clo1_aux go k)
-    | TCase a t1 t2 => interpret_case a (interpret_term1_aux (go_cont' k) t1) (interpret_term1_aux (go_cont' k) t2)
-    | TShift t' => interpret_term1_aux (go_cont' identity) t' (VFun k)
-    | TReset t' => imonad_bind (go_cont' identity t') (interpret_clo1_aux go k)
-    | TCont t' k' => imonad_bind (go_cont' k'  t') (interpret_clo1_aux go k)
-    | _ => imonad_throw OutOfFuel
-    end.
-*)
-
-Definition interpret_app_aux' (go : term -> imonad val) (go_cont : term -> kont -> imonad val) (a1 a2 : imonad val) : imonad val :=
-  imonad_bind a1
-    (fun v1 =>
-       match v1 with
-       | VFun c => imonad_bind a2 (interpret_clo1_aux go c)
-       | VFix c => imonad_bind a2 (interpret_clo2_aux go c v1)
-       | VKont k => interpret_kont_aux' go_cont k a2
-       | _ => imonad_throw (TypeError "")
-       end).
-
-Definition interpret_app' (go : term -> imonad val) (go_cont : term -> kont -> imonad val) (a1 a2 : atom) : imonad val :=
-  interpret_app_aux' go go_cont (interpret_atom a1) (interpret_atom a2).
+  | O => imonad_throw OutOfFuel
+  | S fuel' => interpret_term_kont_aux (interpret_term_kont fuel') t k
+  end.
 
 Definition interpret_term_aux (go : term -> imonad val) (go_kont : term -> kont -> imonad val) : term -> imonad val :=
   fix go' t {struct t} :=
@@ -381,7 +507,16 @@ Definition interpret_term_aux (go : term -> imonad val) (go_kont : term -> kont 
     | TPrim2 p a1 a2 => interpret_prim2 p a1 a2
     | TFun t' => interpret_fun t'
     | TFix t' => interpret_fix t'
-    | TApp a1 a2 => interpret_app' go go_kont a1 a2
+    | TApp a1 a2 => let m1 := interpret_atom a1 in
+                    let m2 := interpret_atom a2 in
+                    imonad_bind m1
+                      (fun v1 =>
+                         match v1 with
+                         | VFun c => imonad_bind m2 (interpret_clo1_aux go c)
+                         | VFix c => imonad_bind m2 (interpret_clo2_aux go c v1)
+                         | VKont k => interpret_kont go_kont k m2
+                         | _ => imonad_throw (TypeError "")
+                         end)
     | TPair a1 a2 => interpret_pair a1 a2
     | TFst a => interpret_fst a
     | TSnd a => interpret_snd a
@@ -393,19 +528,14 @@ Definition interpret_term_aux (go : term -> imonad val) (go_kont : term -> kont 
     | TSet a1 a2 => interpret_set a1 a2
     | TFree a => interpret_free a
     | TShift _ => imonad_throw (ControlError "shift without enclosing reset")
-    | TReset t' => go_kont t' KNil
-    (*| TCont t' k => interpret_term_kont_aux go_kont t' k*)
-    | TCont _ _ => imonad_throw (ControlError "TCont not supported!")
+    | TReset t' => interpret_term_kont_aux go_kont t' KNil
     end.
-
-Definition interpret_term_bot (_ : term) : imonad val :=
-  imonad_throw OutOfFuel.
 
 Fixpoint interpret_term (fuel : nat) (t : term) : imonad val :=
   match fuel with
-  | O => interpret_term_aux interpret_term_bot interpret_term_kont_bot
-  | S fuel' => interpret_term_aux (interpret_term fuel') (interpret_term_kont fuel)
-  end t.
+  | O => imonad_throw OutOfFuel
+  | S fuel' => interpret_term_aux (interpret_term fuel') (interpret_term_kont fuel') t
+  end.
 
 Definition run (fuel : nat) (e : term) : (ierror + val) * istate :=
   interpret_term fuel e ENil istate_empty.
@@ -417,16 +547,17 @@ Definition exec (fuel : nat) (e : term) : istate :=
   snd (run fuel e).
 
 Import Coerce.
+Local Open Scope Z_scope.
 Example f := TReset (TLet
-                       (TPrim2 P2Mul (VInt 6) (VInt 9))
+                       (TPrim2 P2Mul 6 9)
                        (T1 (Var "x")
                           (TLet
                              (TShift (T1 (Var "k") (Var "k")))
                              (T1 (Var "y") (TPrim2 P2Add (Var "x") (Var "y")))))).
-Example fx := TLet f (T1 (Var "f") (TApp (Var "f") (VInt 10))).
-Compute (eval 1 fx).
+Example fx := TLet f (T1 (Var "f") (TApp (Var "f") 10)).
+Compute (eval 2 fx).
 
-Example append :=
+Example append_aux :=
   TFix
     (T2 (Var "f")
        (T1 (Var "xs")
@@ -446,19 +577,64 @@ Example append :=
                                      (TPair (Var "x") (Var "r"))
                                      (T1 (Var "r'") (TInr (Var "r'")))))))))))))).
 
-Fixpoint encode (xs : list Z) : val :=
+Fixpoint encode (xs : list Z) : term :=
   match xs with
-  | nil => VInl VUnit
-  | cons x xs' => VInr (VPair (VInt x) (encode xs'))
+  | nil => TInl AUnit
+  | cons x xs' => TLet (encode xs') (T1 (Var "xs'") (TLet (TPair x (Var "xs'")) (T1 (Var "xs") (TInr (Var "xs")))))
   end.
 
-Example wrap_append v1 :=
-  TReset (TLet append (T1 (Var "append") (TApp (Var "append") v1))).
-Example use_append v1 v2 :=
-  TLet (wrap_append v1)
-    (T1 (Var "f") (TApp (Var "f") v2)).
+Import List.
+Import ListNotations.
 
-Example append1 := use_append (encode nil) (encode (1 :: nil)).
-Example append2 := use_append (encode (1 :: 2 :: 3 :: 4 :: nil)) (encode (4 :: 5 :: 6 :: 7 :: nil)).
+Example append1 xs :=
+  TLet xs (T1 (Var "xs") (TReset (TLet append_aux (T1 (Var "append_aux") (TApp (Var "append_aux") (Var "xs")))))).
 
-Compute (eval 2 (wrap_append (encode (nil)))).
+Example append2 xs ys :=
+  TLet ys (T1 (Var "ys") (TLet (append1 xs) (T1 (Var "append1") (TApp (Var "append1") (Var "ys"))))).
+
+Example ex1_aux := append1 (encode nil).
+Example ex1 := append2 (encode nil) (encode (1 :: nil)).
+Example ex2 := append2 (encode (List.map (fun n => Z.of_nat n) (ListDef.seq 0 1000))) (encode nil).
+
+Example append_direct :=
+  TFix
+    (T2 (Var "f")
+       (T1 (Var "xs")
+          (TFun
+             (T1 (Var "ys")
+                (TCase (Var "xs")
+                   (T1 BAnon (Var "ys"))
+                   (T1 (Var "p")
+                      (TLet
+                         (TFst (Var "p"))
+                         (T1 (Var "x")
+                            (TLet
+                               (TSnd (Var "p"))
+                               (T1 (Var "xs'")
+                                  (TLet
+                                     (TApp (Var "f") (Var "xs'"))
+                                     (T1 (Var "f")
+                                        (TLet
+                                           (TApp (Var "f") (Var "ys"))
+                                           (T1 (Var "r")
+                                              (TLet
+                                                 (TPair (Var "x") (Var "r"))
+                                                 (T1 (Var "r'") (TInr (Var "r'")))))))))))))))))).
+
+Example append xs ys :=
+  TLet xs
+    (T1 (Var "xs")
+       (TLet ys
+          (T1 (Var "ys")
+             (TLet append_direct
+                (T1 (Var "append_aux")
+                   (TLet (TApp (Var "append_aux") (Var "xs"))
+                      (T1 (Var "f") (TApp (Var "f") (Var "ys"))))))))).
+
+Definition xs := encode (List.map (fun n => Z.of_nat n) (ListDef.seq 0 1000)).
+
+Example ex3 := append xs (encode nil).
+
+Compute (eval 10 ex1_aux).
+Time Compute (eval 10 ex1).
+Time Compute (interpret_term 1000 xs ENil istate_empty).
